theories/rules/run.v
@@ -1,5 +1,5 @@
 From machine_program_logic.program_logic Require Import weakestpre.
-From HypVeri Require Import lifting rules.rules_base.
+From HypVeri Require Import machine_extra lifting rules.rules_base.
 From HypVeri.algebra Require Import base reg mem pagetable base_extra.
 From HypVeri.lang Require Import lang_extra reg_extra current_extra.
 Require Import stdpp.fin.
@@ -11,34 +11,33 @@ Context `{hypparams:HypervisorParameters}.
   
 Context `{vmG: !gen_VMG Σ}.
 
-Lemma run {E z w1 w2 w3 q R R' Q P P' i'} ai i :
-  let T := (▷ (PC @@ z ->r ai)
+Lemma run {E w1 w2 w3 q s R R' Q P P'} ai i :
+  let T := (▷ (PC @@ V0 ->r ai)
             ∗ ▷ (ai ->a w1)
-            ∗ ▷ (z -@{q}A> (tpa ai))
-            ∗ ▷ (R0 @@ z ->r w2)
-            ∗ ▷ (R1 @@ z ->r w3))%I
+            ∗ ▷ (V0 -@{q}A> [s])
+            ∗ ▷ (R0 @@ V0 ->r w2)
+            ∗ ▷ (R1 @@ V0 ->r w3))%I
   in
-  let T' := ((PC @@ z ->r (ai ^+ 1)%f)
+  let T' := ((PC @@ V0 ->r (ai ^+ 1)%f)
                ∗ (ai ->a w1)
-               ∗ (z -@{q}A> (tpa ai))
-               ∗ (R0 @@ z ->r w2)
-               ∗ (R1 @@ z ->r w3))%I
+               ∗ (V0 -@{q}A> [s])
+               ∗ (R0 @@ V0 ->r w2)
+               ∗ (R1 @@ V0 ->r w3))%I
   in
+  (tpa ai) ∈ s ->
+  i ≠ V0 ->
   decode_instruction w1 = Some Hvc ->
-  fin_to_nat z = 0 ->
-  fin_to_nat i = i' ->
-  i' ≠ 0 ->
   decode_hvc_func w2 = Some Run ->
   decode_vmid w3 = Some i ->
-  {SS{{ T ∗ ▷ (VMProp i (Q ∗ VMProp z P' (1/2)%Qp) (1/2)%Qp)
-          ∗ ▷ (VMProp z P 1%Qp)
-          ∗ ▷ (T' ∗ R -∗ (Q ∗ R')) 
+  {SS{{ T ∗ ▷ (VMProp i (Q) (1/2)%Qp)
+          ∗ ▷ (VMProp V0 P 1%Qp)
+          ∗ ▷ (T' ∗ R ∗ VMProp V0 P' (1/2)%Qp -∗ (Q ∗ R'))
           ∗ ▷ R }}}
-    ExecI @ z ;E
-    {{{ RET (true, ExecI); R' ∗ VMProp z P' (1/2)%Qp}}}.
+    ExecI @ V0 ;E
+    {{{ RET (true, ExecI); R' ∗ VMProp V0 P' (1/2)%Qp}}}.
 Proof.
   simpl.
-  iIntros (Hdecode Hz Hi Hiz Hhvc Hvmid ϕ) "[(>Hpc & >Hapc & >Hacc & >Hr0 & >Hr1) (HPropi & HPropz & Himpl & HR)] Hϕ".
+  iIntros (Hin Hneq_v Hdecode Hhvc Hvmid ϕ) "[(>Hpc & >Hapc & >Hacc & >Hr0 & >Hr1) (HPropi & HPropz & Himpl & HR)] Hϕ".
   iApply (sswp_lift_atomic_step ExecI); [done|].
   iIntros (n σ1) "%Hsche Hσ".
   rewrite /scheduled in Hsche.
@@ -50,30 +49,32 @@ Proof.
   iModIntro.
   iDestruct "Hσ" as "(%Hneq & Hmemown & Hregown & Hrx & Hown & Hmb & Haccessown & Hrest)".
   (* valid regs *)
-  iDestruct (gen_reg_valid1 PC z ai Hcur with "Hregown Hpc") as "%Hpc".
-  iDestruct (gen_reg_valid1 R0 z w2 Hcur with "Hregown Hr0") as "%Hr0".
-  iDestruct (gen_reg_valid1 R1 z w3 Hcur with "Hregown Hr1") as "%Hr1".
+  iDestruct (gen_reg_valid1 PC V0 ai Hcur with "Hregown Hpc") as "%Hpc".
+  iDestruct (gen_reg_valid1 R0 V0 w2 Hcur with "Hregown Hr0") as "%Hr0".
+  iDestruct (gen_reg_valid1 R1 V0 w3 Hcur with "Hregown Hr1") as "%Hr1".
   (* valid pt *)
-  iDestruct (access_agree_check_true (tpa ai)  with "Haccessown Hacc") as %Hacc;first set_solver +.
+  iDestruct (access_agree_check_true (tpa ai)  with "Haccessown Hacc") as %Hacc;first exact Hin.
   (* valid mem *)
   iDestruct (gen_mem_valid ai w1 with "Hmemown Hapc") as "%Hmem".
   iSplit.
   - (* reducible *)
     iPureIntro.
-    apply (reducible_normal z Hvc ai w1);eauto.
+    apply (reducible_normal V0 Hvc ai w1);eauto.
   - iModIntro.
     iIntros (m2 σ2) "[%U PAuth] %HstepP".
-    apply (step_ExecI_normal z Hvc ai w1) in HstepP; eauto.
+    apply (step_ExecI_normal V0 Hvc ai w1) in HstepP; eauto.
     remember (exec Hvc σ1) as c2 eqn:Heqc2.
     rewrite /exec /hvc in Heqc2; eauto.
     rewrite  Hr0 Hhvc /run Hr1 in Heqc2.
     simpl in Heqc2.
     rewrite /unpack_hvc_result_yield Hvmid in Heqc2.
     simpl in Heqc2.
-    rewrite /is_primary Hcur Hz in Heqc2.
-    destruct (0 =? 0) eqn:Hvmz; [|done].
+    rewrite /is_primary Hcur in Heqc2.
     destruct HstepP as [Hstep1 Hstep2].
-    simplify_eq.
+    case_bool_decide;last done.
+    subst c2.
+    simpl in Hstep1, Hstep2.
+    subst σ2 m2.
     simpl.
     rewrite /gen_vm_interp /update_incr_PC.
     rewrite (preserve_get_mb_gmap σ1).
@@ -94,11 +95,10 @@ Proof.
     all: try rewrite p_upd_id_trans p_upd_pc_trans //.
     rewrite p_upd_id_mem p_upd_pc_mem.
     iFrame "Hrest Hrx Hmb Hmemown Haccessown Hown".
-    iDestruct ((gen_reg_update1_global PC (get_current_vm σ1) ai (ai ^+ 1)%f) with "Hregown Hpc") as "HpcUpd".
+    iDestruct ((gen_reg_update1_global PC V0 ai (ai ^+ 1)%f) with "Hregown Hpc") as "HpcUpd".
     rewrite (preserve_get_reg_gmap (update_offset_PC σ1 1) (update_current_vmid _ _));last rewrite p_upd_id_reg //.
-    rewrite ->(update_offset_PC_update_PC1 _ (get_current_vm σ1) ai 1); auto.
-    + rewrite Hz.
-      iDestruct (VMProp_update 0 U P P' with "PAuth HPropz") as "HTemp".
+    rewrite ->(update_offset_PC_update_PC1 _ V0 ai 1); auto.
+    + iDestruct (VMProp_update V0 U P P' with "PAuth HPropz") as "HTemp".
       iMod "HpcUpd".
       iMod "HTemp".
       iDestruct "HTemp" as "[PAuth HPropz]".
@@ -113,20 +113,26 @@ Proof.
                 (λ id : vmid,
                         base.negb (scheduled σ1 id) &&
                         scheduled (update_current_vmid (update_offset_PC σ1 1) i) id = true)
-                (seq 0 vm_count) = [fin_to_nat i]) as ->.
+                (seq 0 n) = [fin_to_nat i]) as ->.
       {
-        rewrite /scheduled /machine.scheduler //= /scheduler Hz.
+        rewrite /scheduled /machine.scheduler Hneq //= /scheduler.
         rewrite /update_current_vmid //=.
         pose proof (NoDup_seq 0 vm_count) as ND.
         pose proof (NoDup_singleton ((@fin_to_nat (@vm_count H) i))) as ND'.
-        set f := (λ id : nat, base.negb (bool_decide (0 = id)) && bool_decide ((@fin_to_nat (@vm_count H) i) = id) = true).
+        set f := (λ id : nat, base.negb (bool_decide ((@fin_to_nat (@vm_count H) σ1.1.1.2) = id)) && bool_decide ((@fin_to_nat (@vm_count H) i) = id) = true).
         pose proof (NoDup_filter f _ ND) as ND''.
         assert (f i) as Prf.
         {
           subst f.
           simpl.
           unfold base.negb.
-          repeat case_bool_decide; done.
+          repeat case_bool_decide; eauto.
+          rewrite Hcur in H1.
+          exfalso.
+          apply Hneq_v.
+          symmetry.
+          apply fin_to_nat_inj.
+          done.
         }
         assert (In (@fin_to_nat (@vm_count H) i) (seq 0 vm_count)) as Prf'.
         {
@@ -171,12 +177,12 @@ Proof.
         - intros T.
           rewrite ->elem_of_list_singleton.
           rewrite ->elem_of_list_In in T.
-          destruct (decide (x' = i)) as [? | n]; auto.
+          destruct (decide (x' = i)) as [? | n']; auto.
           exfalso.
-          by apply (excl x' n).
+          by apply (excl x' n').
       }
       iSimpl.
-      assert ((negb (scheduled (update_current_vmid (update_offset_PC σ1 1) i) 0) && true = true)) as ->.
+      assert ((negb (scheduled (update_current_vmid (update_offset_PC σ1 1) i) V0) && true = true)) as ->.
       {
         rewrite andb_true_r.
         rewrite /scheduled /machine.scheduler //= /scheduler.
@@ -184,18 +190,18 @@ Proof.
         apply eq_true_not_negb.
         intros c.
         rewrite ->bool_decide_eq_true in c.
-        by apply Hiz.
+        apply Hneq_v.
+        apply fin_to_nat_inj.
+        done.
       }
       iDestruct (VMProp_split with "HPropz") as "[HPropz1 HPropz2]".
-      iDestruct ("Himpl" with "[Hpc Hapc Hacc Hr0 Hr1 HR]") as "[Q R']".
+      iDestruct ("Himpl" with "[Hpc Hapc Hacc Hr0 Hr1 HR HPropz1]") as "[Q R']".
       iFrame.
-      iSplitR "Hϕ R' HPropz1".
+      iSplitR "Hϕ R' HPropz2".
       iSplit; last done.
-      iExists (Q ∗ VMProp 0 P' (1 / 2))%I.      
-      iFrame "HPropi".
-      iNext.
-      iFrame "HPropz2 Q".
-      iApply ("Hϕ" with "[R' HPropz1]").
+      iExists (Q)%I.
+      iFrame.
+      iApply ("Hϕ" with "[R' HPropz2]").
       iFrame.
     + apply get_reg_gmap_get_reg_Some; auto.
 Qed.
