theories/rules/yield.v
@@ -1,6 +1,6 @@
 From machine_program_logic.program_logic Require Import weakestpre.
-From HypVeri Require Import lifting rules.rules_base.
-From HypVeri Require Import base reg mem pagetable base_extra.
+From HypVeri Require Import machine_extra lifting rules.rules_base.
+From HypVeri.algebra Require Import base reg mem pagetable base_extra.
 From HypVeri.lang Require Import lang_extra reg_extra current_extra.
 Require Import stdpp.fin.
 Require Import stdpp.listset_nodup.
@@ -10,35 +10,34 @@ Section yield.
 Context `{hypparams:HypervisorParameters}.
 Context `{vmG: !gen_VMG Σ}.
 
-Lemma yield {E z i w1 w2 a_ b_ q R R' Q P P' i'} ai :
+Lemma yield {E w1 w2 a_ b_ q s R R' Q P P' i} ai :
   let T := (▷ (PC @@ i ->r ai)
               ∗ ▷ (ai ->a w1)
-              ∗ ▷ (i -@{q}A> (tpa ai))
+              ∗ ▷ (i -@{q}A> [s])
               ∗ ▷ (R0 @@ i ->r w2)
-              ∗ ▷ (R0 @@ z ->r a_)
-              ∗ ▷ (R1 @@ z ->r b_))%I
+              ∗ ▷ (R0 @@ V0 ->r a_)
+              ∗ ▷ (R1 @@ V0 ->r b_))%I
   in
   let T' := ((PC @@ i ->r (ai ^+ 1)%f)
                ∗ (ai ->a w1)
-               ∗ (i -@{q}A> (tpa ai))
+               ∗ (i -@{q}A> [s])
                ∗ (R0 @@ i ->r w2)
-               ∗ (R0 @@ z ->r (encode_hvc_func Yield))
-               ∗ (R1 @@ z ->r (encode_vmid i)))%I
+               ∗ (R0 @@ V0 ->r (encode_hvc_func Yield))
+               ∗ (R1 @@ V0 ->r (encode_vmid i)))%I
   in
+  (tpa ai) ∈ s ->
+  i ≠ V0 ->
   decode_instruction w1 = Some Hvc ->
-  fin_to_nat z = 0 ->
-  fin_to_nat i = i' ->
-  i' ≠ 0 ->
   decode_hvc_func w2 = Some Yield ->
-  {SS{{ T ∗ ▷ (VMProp z (Q ∗ VMProp i P' (1/2)%Qp) (1/2)%Qp)
+  {SS{{ T ∗ ▷ (VMProp V0 (Q ) (1/2)%Qp)
           ∗ ▷ (VMProp i P 1%Qp)
-          ∗ ▷ (T' ∗ R -∗ (Q ∗ R'))
+          ∗ ▷ (T' ∗ R ∗ VMProp i P' (1/2)%Qp -∗ (Q ∗ R'))
           ∗ ▷ R }}}
     ExecI @ i;E
     {{{ RET (true, ExecI); R' ∗ VMProp i P' (1/2)%Qp }}}.
 Proof.
   simpl.
-  iIntros (Hdecode Hz Hi Hiz Hhvc ϕ) "[(>Hpc & >Hapc & >Hacc & >Hr0 & >Hr0' & >Hr1) (HPropz & HPropi & Himpl & HR)] Hϕ".
+  iIntros (Hin Hneq_v Hdecode Hhvc ϕ) "[(>Hpc & >Hapc & >Hacc & >Hr0 & >Hr0' & >Hr1) (HPropz & HPropi & Himpl & HR)] Hϕ".
   iApply (sswp_lift_atomic_step ExecI); [done|].
   iIntros (n σ1) "%Hsche Hσ".
   rewrite /scheduled in Hsche.
@@ -52,10 +51,10 @@ Proof.
   (* valid regs *)
   iDestruct (gen_reg_valid1 PC i ai Hcur with "Hregown Hpc") as "%Hpc".
   iDestruct (gen_reg_valid1 R0 i w2 Hcur with "Hregown Hr0") as "%Hr0".
-  iDestruct (gen_reg_valid_global1 R0 z a_ with "Hregown Hr0'") as "%Hr0'".
-  iDestruct (gen_reg_valid_global1 R1 z b_ with "Hregown Hr1") as "%Hr1".
+  iDestruct (gen_reg_valid_global1 R0 V0 a_ with "Hregown Hr0'") as "%Hr0'".
+  iDestruct (gen_reg_valid_global1 R1 V0 b_ with "Hregown Hr1") as "%Hr1".
   (* valid pt *)
-  iDestruct (access_agree_check_true with "Haccessown Hacc") as %Hacc; first (apply elem_of_singleton;reflexivity).
+  iDestruct (access_agree_check_true with "Haccessown Hacc") as %Hacc;first exact Hin.
   (* valid mem *)
   iDestruct (gen_mem_valid ai w1 with "Hmemown Hapc") as "%Hmem".
   iSplit.
@@ -69,19 +68,15 @@ Proof.
     rewrite /exec /hvc in Heqc2; eauto.
     rewrite  Hr0 Hhvc /yield in Heqc2.
     rewrite /is_primary /update_reg p_upd_reg_current_vm Hcur in Heqc2.
-    destruct (i =? 0) eqn:Hi0.
-    + rewrite <-(reflect_iff (fin_to_nat i = 0) (i =? 0) (Nat.eqb_spec (fin_to_nat i) 0)) in Hi0.
-      exfalso.
-      apply Hiz.
-      solve_finz.
+    destruct (decide (i = V0)).
+    + exfalso.
+      by apply Hneq_v.
     + destruct HstepP as [Hstep1 Hstep2].
       simplify_eq.
-      assert (Hzeq : z = nat_to_fin vm_count_pos).
+      assert (bool_decide (σ1.1.1.2 = V0) = false) as ->.
       {
-        apply fin_to_nat_inj.
-        rewrite fin_to_nat_to_fin; auto.
+        rewrite bool_decide_eq_false //.
       }
-      rewrite <-Hzeq.
       simpl.
       rewrite /gen_vm_interp /update_incr_PC.
       rewrite (preserve_get_mb_gmap σ1).
@@ -103,18 +98,18 @@ Proof.
       rewrite p_upd_id_mem p_upd_pc_mem.
       iFrame "Hrx Hmb Hown Hrest".
       iDestruct (gen_reg_update_Sep
-                  {[(R0, z):= a_;
-                    (R1, z):= b_;
+                  {[(R0, V0):= a_;
+                    (R1, V0):= b_;
                     (PC, get_current_vm σ1) := ai]}
-                  {[(R0, z):= of_imm (encode_hvc_func Yield);
-                    (R1, z):= of_imm (encode_vmid (get_current_vm σ1));
+                  {[(R0, V0):= of_imm (encode_hvc_func Yield);
+                    (R1, V0):= of_imm (encode_vmid (get_current_vm σ1));
                     (PC, get_current_vm σ1) := (ai ^+ 1)%f]} with "Hregown [Hr0' Hr1 Hpc]") as ">[Hreg Hr01pc]"; [set_solver | |].
       * rewrite !big_sepM_insert ?big_sepM_empty; eauto; [iFrame | |].
         apply lookup_insert_None; split; eauto; intros P; by inversion P.
         apply lookup_insert_None. split; [apply lookup_insert_None; split; eauto; intros P; by inversion P |]; eauto; intros P; by inversion P.
       * rewrite !big_sepM_insert ?big_sepM_empty; eauto.
         iDestruct "Hr01pc" as "(Hr0' & Hr1' & Hpc' & _)".
-        assert ((negb (scheduled (update_current_vmid (update_offset_PC (update_reg_global (update_reg_global σ1 z R0 (encode_hvc_func Yield)) z R1 (encode_vmid (get_current_vm σ1))) 1) z) (get_current_vm σ1)) && true = true)) as ->.
+        assert ((negb (scheduled (update_current_vmid (update_offset_PC (update_reg_global (update_reg_global σ1 V0 R0 (encode_hvc_func Yield)) V0 R1 (encode_vmid (get_current_vm σ1))) 1) V0) (get_current_vm σ1)) && true = true)) as ->.
         {
           rewrite andb_true_r.
           rewrite /scheduled /machine.scheduler //= /scheduler.
@@ -122,57 +117,61 @@ Proof.
           apply eq_true_not_negb.
           intros c.
           rewrite ->bool_decide_eq_true in c.
-          apply Hiz.
-          by rewrite <-c.
+          inversion c.
+          apply n0.
+          symmetry.
+          apply fin_to_nat_inj.
+          done.
         }
         rewrite /just_scheduled_vms /just_scheduled.
         assert (filter
                   (λ id : vmid,
-                          base.negb (scheduled σ1 id) && scheduled (update_current_vmid (update_offset_PC (update_reg_global (update_reg_global σ1 z R0 (encode_hvc_func Yield)) z R1 (encode_vmid (get_current_vm σ1))) 1) z) id = true)
-                  (seq 0 vm_count) = [fin_to_nat z]) as ->.
+                          base.negb (scheduled σ1 id) && scheduled (update_current_vmid (update_offset_PC (update_reg_global (update_reg_global σ1 V0 R0 (encode_hvc_func Yield)) V0 R1 (encode_vmid (get_current_vm σ1))) 1) V0) id = true)
+                  (seq 0 vm_count) = [0]) as ->.
         {
-        rewrite /scheduled /machine.scheduler //= /scheduler Hz.
+        rewrite /scheduled /machine.scheduler //= /scheduler.
         rewrite /update_current_vmid //=.
         pose proof (NoDup_seq 0 vm_count) as ND.
-        pose proof (NoDup_singleton ((@fin_to_nat (@vm_count H) z))) as ND'.
-        set f := (λ id : nat, base.negb (bool_decide ((@fin_to_nat (@vm_count H) σ1.1.1.2) = id)) && bool_decide (0 = id) = true).
+        pose proof (NoDup_singleton 0) as ND'.
+        set f := (λ id : nat, base.negb (bool_decide ((@fin_to_nat (@vm_count H) σ1.1.1.2) = id)) && bool_decide (fin_to_nat V0 = id) = true).
         pose proof (NoDup_filter f _ ND) as ND''.
-        assert (f z) as Prf.
+        assert (f 0) as Prf.
         {
           subst f.
           simpl.
           unfold base.negb.
-          repeat case_bool_decide.
+          repeat case_bool_decide;eauto.
           exfalso.
-          apply Hiz.
-          (* FIXME *)
-          by rewrite H1.
-          exfalso.
-          apply H1.
-          by rewrite Hz.
+          apply n0.
+          apply fin_to_nat_inj.
+          rewrite H0.
+          symmetry.
           done.
           exfalso.
           apply H1.
-          by rewrite Hz.
+          apply V0eq.
+          exfalso.
+          apply H1.
+          apply V0eq.
         }
-        assert (In (@fin_to_nat (@vm_count H) z) (seq 0 vm_count)) as Prf'.
+
+        assert (In 0 (seq 0 vm_count)) as Prf'.
         {
           rewrite <-elem_of_list_In.
           rewrite elem_of_seq.
           split.
           - solve_finz.
           - rewrite plus_O_n.
-            pose proof (fin_to_nat_lt z).
-            auto.
+            apply vm_count_pos.
         }
         rewrite <-elem_of_list_In in Prf'.
-        assert (In (@fin_to_nat (@vm_count H) z) (filter f (seq 0 vm_count))) as Prf''.
+        assert (In 0 (filter f (seq 0 vm_count))) as Prf''.
         {
           rewrite <-elem_of_list_In.
-          by apply (iffRL (elem_of_list_filter f (seq 0 vm_count) z)).
+          by apply (iffRL (elem_of_list_filter f (seq 0 vm_count) 0)).
         }
         rewrite <-elem_of_list_In in Prf''.
-        assert (forall x, x ≠ (@fin_to_nat (@vm_count H) z) -> not (In x (filter f (seq 0 vm_count)))) as excl.
+        assert (forall x, x ≠ 0 -> not (In x (filter f (seq 0 vm_count)))) as excl.
         {
           intros x neq c.
           rewrite <-elem_of_list_In in c.
@@ -187,26 +186,24 @@ Proof.
             apply neq.
             rewrite ->bool_decide_eq_true in c'.
             rewrite <-c'.
-            done.
+            apply V0eq.
         }
         apply Permutation_length_1_inv.
         apply NoDup_Permutation; auto.
-        by rewrite <-Hz.
         intros x'.
         split.
         - intros T.
           rewrite ->elem_of_list_singleton in T.
-          rewrite Hz in Prf''.
           by rewrite T.
         - intros T.
           rewrite ->elem_of_list_singleton.
           rewrite ->elem_of_list_In in T.
-          destruct (decide (x' = z)) as [? | n].
-          by rewrite Hz in e.
+          destruct (decide (x' = 0)) as [? | n].
+          done.
           exfalso.
           by apply (excl x' n).
       }
-        set σ1' := (X in (update_current_vmid X z)).
+        set σ1' := (X in (update_current_vmid X V0)).
         rewrite (preserve_get_reg_gmap σ1' (update_current_vmid _ _)); last rewrite p_upd_id_reg //.
         rewrite /σ1'.
         rewrite ->(update_offset_PC_update_PC1 _ (get_current_vm σ1) ai 1); auto.
@@ -221,14 +218,14 @@ Proof.
            iSplit; first done.
            rewrite 2!update_reg_global_update_reg.
            rewrite !insert_union_singleton_l.
-           rewrite (map_union_comm {[(R1, z) := of_imm (encode_vmid σ1.1.1.2)]} {[(PC, σ1.1.1.2) := (ai ^+ 1)%f]}).
+           rewrite (map_union_comm {[(R1, V0) := of_imm (encode_vmid σ1.1.1.2)]} {[(PC, σ1.1.1.2) := (ai ^+ 1)%f]}).
            rewrite map_union_assoc.
-           rewrite (map_union_comm {[(R0, z) := of_imm (encode_hvc_func Yield)]} {[(PC, σ1.1.1.2) := (ai ^+ 1)%f]}).
+           rewrite (map_union_comm {[(R0, V0) := of_imm (encode_hvc_func Yield)]} {[(PC, σ1.1.1.2) := (ai ^+ 1)%f]}).
            rewrite <-(map_union_assoc {[(PC, σ1.1.1.2) := (ai ^+ 1)%f]}
-                                      {[(R0, z) := of_imm (encode_hvc_func Yield)]}
-                                      {[(R1, z) := of_imm (encode_vmid σ1.1.1.2)]}).
-           rewrite (map_union_comm {[(R0, z) := of_imm (encode_hvc_func Yield )]}
-                                   {[(R1, z) := of_imm (encode_vmid σ1.1.1.2)]}).
+                                      {[(R0, V0) := of_imm (encode_hvc_func Yield)]}
+                                      {[(R1, V0) := of_imm (encode_vmid σ1.1.1.2)]}).
+           rewrite (map_union_comm {[(R0, V0) := of_imm (encode_hvc_func Yield )]}
+                                   {[(R1, V0) := of_imm (encode_vmid σ1.1.1.2)]}).
            rewrite !map_union_assoc.
            iAssumption.
            by rewrite map_disjoint_singleton_r lookup_singleton_None.
@@ -238,30 +235,23 @@ Proof.
            eapply mk_is_Some; rewrite lookup_insert_Some;
              right; split; [done | rewrite get_reg_gmap_lookup_Some; eauto].
            eapply mk_is_Some; rewrite get_reg_gmap_lookup_Some; eauto.
-           iDestruct ("Himpl" with "[Hpc' Hapc Hacc Hr0 Hr0' Hr1' HR]") as "[Q R']".
-           iFrame.
            iDestruct (VMProp_split with "HPropi") as "[HPropi1 HPropi2]".
-           iSplitR "Hϕ R' HPropi1".
+           iDestruct ("Himpl" with "[Hpc' Hapc Hacc Hr0 Hr0' Hr1' HR HPropi1]") as "[Q R']".
+           iFrame.
+           iSplitR "Hϕ R' HPropi2".
            simpl.
            iSplit; last done.
-           iExists (Q ∗ VMProp σ1.1.1.2 P' (1 / 2))%I.
+           iExists (Q)%I.
+           rewrite V0eq.
            iFrame.
-           iApply ("Hϕ" with "[R' HPropi1]").
+           iApply ("Hϕ" with "[R' HPropi2]").
            iFrame.
         -- apply get_reg_gmap_get_reg_Some; auto.
            apply get_reg_global_update_reg_global_ne_vmid.
            rewrite p_upd_reg_current_vm; auto.
            rewrite p_upd_reg_current_vm; auto.
-           intros c.
-           apply Hiz.
-           rewrite <-c.
-           by rewrite Hz.
-           apply get_reg_global_update_reg_global_ne_vmid.           
-           rewrite 2!p_upd_reg_current_vm; auto.
-           intros c.
-           apply Hiz.
-           rewrite <-c.
-           by rewrite Hz.
+           apply get_reg_global_update_reg_global_ne_vmid.
+           rewrite p_upd_reg_current_vm; auto.
            rewrite p_upd_reg_current_vm; auto.
         -- apply lookup_insert_None; split; eauto; intros P; by inversion P.
         -- apply lookup_insert_None. split; [apply lookup_insert_None; split; eauto; intros P; by inversion P |]; eauto; intros P; by inversion P.
